Test/Builtin/attributes.mlir
@@ -2,26 +2,26 @@
 
 "builtin.module"() ({
 ^bb0():
-  %3 = "test.test"() <{str = "hello world"}> : () -> i32
-  %4 = "test.test"() <{empty = ""}> : () -> i32
-  %5 = "test.test"() <{escaped = "line1\nline2\ttab"}> : () -> i32
-  %6 = "test.test"() <{unregistered = #unregistered.dialect<foo 3 + 2>}> : () -> i32
-  %7 = "test.test"() <{u = unit}> : () -> i32
-  %8 = "test.test"() <{u}> : () -> i32
-  %9 = "test.test"() <{dict = {a = 0 : i32, b = "hello"}}> : () -> i32
-  %10 = "test.test"() <{empty_dict = {}}> : () -> i32
-  %11 = "test.test"() <{dict_unit = {x, y}}> : () -> i32
+  %3 = "test.test"() {str = "hello world"} : () -> i32
+  %4 = "test.test"() {empty = ""} : () -> i32
+  %5 = "test.test"() {escaped = "line1\nline2\ttab"} : () -> i32
+  %6 = "test.test"() {unregistered = #unregistered.dialect<foo 3 + 2>} : () -> i32
+  %7 = "test.test"() {u = unit} : () -> i32
+  %8 = "test.test"() {u} : () -> i32
+  %9 = "test.test"() {dict = {a = 0 : i32, b = "hello"}} : () -> i32
+  %10 = "test.test"() {empty_dict = {}} : () -> i32
+  %11 = "test.test"() {dict_unit = {x, y}} : () -> i32
 }) : () -> ()
 
 // CHECK-NEXT: "builtin.module"() ({
 // CHECK-NEXT:   ^{{.*}}():
-// CHECK-NEXT:     %{{.*}} = "test.test"() : () -> i32
-// CHECK-NEXT:     %{{.*}} = "test.test"() : () -> i32
-// CHECK-NEXT:     %{{.*}} = "test.test"() : () -> i32
-// CHECK-NEXT:     %{{.*}} = "test.test"() : () -> i32
-// CHECK-NEXT:     %{{.*}} = "test.test"() : () -> i32
-// CHECK-NEXT:     %{{.*}} = "test.test"() : () -> i32
-// CHECK-NEXT:     %{{.*}} = "test.test"() : () -> i32
-// CHECK-NEXT:     %{{.*}} = "test.test"() : () -> i32
-// CHECK-NEXT:     %{{.*}} = "test.test"() : () -> i32
+// CHECK-NEXT:     %{{.*}} = "test.test"() { str = "hello world" } : () -> i32
+// CHECK-NEXT:     %{{.*}} = "test.test"() { empty = "" } : () -> i32
+// CHECK-NEXT:     %{{.*}} = "test.test"() { escaped = "line1\nline2\ttab" } : () -> i32
+// CHECK-NEXT:     %{{.*}} = "test.test"() { unregistered = #unregistered.dialect<foo 3 + 2> } : () -> i32
+// CHECK-NEXT:     %{{.*}} = "test.test"() { u } : () -> i32
+// CHECK-NEXT:     %{{.*}} = "test.test"() { u } : () -> i32
+// CHECK-NEXT:     %{{.*}} = "test.test"() { dict = { a = 0 : i32, b = "hello" } } : () -> i32
+// CHECK-NEXT:     %{{.*}} = "test.test"() { empty_dict = {} } : () -> i32
+// CHECK-NEXT:     %{{.*}} = "test.test"() { dict_unit = { x, y } } : () -> i32
 // CHECK-NEXT: }) : () -> ()
