Test/Parsing/attributes.mlir
@@ -2,5 +2,5 @@
 
 "builtin.module"() ({
     "test.test"() { test = 23 : i32, "fo/no" = 1 : i32 } : () -> ()
-    // CHECK:     "test.test"() : () -> ()
+    // CHECK:     "test.test"() { fo/no = 1 : i32, test = 23 : i32 } : () -> ()
 }) : () -> ()
